more substring and sequence lemmas

leetcode/invertBinaryTree.dfy
@@ -1,16 +1,16 @@
 /**
  * https://leetcode.com/problems/invert-binary-tree/description/
  * Definition for a binary tree node.
- * class TreeNode {
- *     val: number
- *     left: TreeNode | null
- *     right: TreeNode | null
- *     constructor(val?: number, left?: TreeNode | null, right?: TreeNode | null) {
- *         this.val = (val===undefined ? 0 : val)
- *         this.left = (left===undefined ? null : left)
- *         this.right = (right===undefined ? null : right)
- *     }
- * }
+ class TreeNode {
+     val: number
+     left: TreeNode | null
+     right: TreeNode | null
+     constructor(val?: number, left?: TreeNode | null, right?: TreeNode | null) {
+         this.val = (val===undefined ? 0 : val)
+         this.left = (left===undefined ? null : left)
+         this.right = (right===undefined ? null : right)
+     }
+ }
 
 function invertTree(root: TreeNode | null): TreeNode | null {
     if(root == null) return null;
@@ -21,7 +21,8 @@ function invertTree(root: TreeNode | null): TreeNode | null {
     return root;
 };
  */
-
+include "../lib/seq.dfy"
+import opened Seq
 class TreeNode {
     var val: int;
     var left: TreeNode?;
@@ -69,6 +70,14 @@ class TreeNode {
         && (this.right == null && this.left == null ==> this.repr == {this})
     }
 
+    predicate iterativeValid()
+        reads this, repr
+        decreases repr
+        requires this.Valid()
+    {
+        forall x :: x in PreorderTraversal(this) ==> x in repr
+    }
+
     method  invertBinaryTree() returns (newRoot: TreeNode?)
         modifies this.repr
         requires this.Valid()
@@ -90,6 +99,322 @@ class TreeNode {
         return this;
     }
 
+
+}
+
+datatype Tree = Node(val: int, left: Tree, right: Tree) | Nil
+
+predicate injectiveSeq<A>(s: seq<A>) {
+    forall x,y :: x != y && 0 <= x < y < |s| ==> s[x] != s[y]
+}
+
+function method PreorderTraversal(root: TreeNode): seq<TreeNode>
+    reads root.repr
+    requires root.Valid()
+    // ensures forall x :: x in PreorderTraversal(root) ==> x.Valid()
+    ensures forall x :: x in root.repr ==> x in PreorderTraversal(root)
+    ensures forall k :: 0 <= k < |PreorderTraversal(root)| ==> PreorderTraversal(root)[k] in root.repr && PreorderTraversal(root)[k].Valid()
+    ensures injectiveSeq(PreorderTraversal(root))
+    ensures forall k :: 0 <= k < |PreorderTraversal(root)| ==> PreorderTraversal(root)[k] in root.repr
+    // ensures forall k :: 0 <= k < |PreorderTraversal(root)| ==> forall child :: child in PreorderTraversal(root)[k].repr && child != child in PreorderTraversal(root)[k] ==> exists j :: k < j < |PreorderTraversal(root)| && PreorderTraversal(root)[j] == child
+{
+   if root.left != null && root.right != null then [root]+PreorderTraversal(root.left)+PreorderTraversal(root.right) else if root.left != null then [root]+PreorderTraversal(root.left) else if root.right != null then [root]+PreorderTraversal(root.right) else [root]
+}
+
+function method TreePreorderTraversal(root: Tree): seq<Tree>
+    // ensures forall x :: x in TreePreorderTraversal(root) ==> x != Nil
+    // ensures forall x :: x in TreePreorderTraversal(root) ==> x != Nil && (x == root || x in TreePreorderTraversal(root.left) || x in TreePreorderTraversal(root.right))
+    // ensures forall x :: x in root.repr ==> x in PreorderTraversal(root)
+    // ensures injectiveSeq(TreePreorderTraversal(root))
+    // ensures forall k :: 0 <= k < |TreePreorderTraversal(root)| ==> TreePreorderTraversal(root)[k] in root.repr
+    // ensures forall k :: 0 <= k < |PreorderTraversal(root)| ==> forall child :: child in PreorderTraversal(root)[k].repr && child != child in PreorderTraversal(root)[k] ==> exists j :: k < j < |PreorderTraversal(root)| && PreorderTraversal(root)[j] == child
+{
+   if root == Nil then [] else if root.left != Nil && root.right != Nil then [root]+TreePreorderTraversal(root.left)+TreePreorderTraversal(root.right) else if root.left != Nil then [root]+TreePreorderTraversal(root.left) else if root.right != Nil then [root]+TreePreorderTraversal(root.right) else [root]
+}
+
+lemma NoNil(root: Tree)
+    ensures forall x :: x in TreePreorderTraversal(root) ==> x != Nil
+{
+
+}
+
+lemma tpt(root: Tree)
+    ensures forall x :: x in TreePreorderTraversal(root) ==> x != Nil
+    ensures forall x :: x in TreePreorderTraversal(root) ==> x != Nil && (x == root || x in TreePreorderTraversal(root.left) || x in TreePreorderTraversal(root.right))
+{
+
+}
+
+lemma AllChildTraversalElementsInRoot(root: Tree, elem: Tree)
+    requires elem in TreePreorderTraversal(root)
+    ensures forall child :: child in TreePreorderTraversal(elem) ==> child in TreePreorderTraversal(root)
+{
+
+}
+
+lemma TreePreorderTraversalSubstrings(root: Tree)
+    requires root != Nil
+    ensures root.left != Nil ==> isSubstring(TreePreorderTraversal(root.left), TreePreorderTraversal(root))
+    ensures root.right != Nil ==> isSubstring(TreePreorderTraversal(root.right), TreePreorderTraversal(root))
+{
+   if root.left != Nil && root.right != Nil {
+    calc {
+        TreePreorderTraversal(root);
+        [root]+TreePreorderTraversal(root.left)+TreePreorderTraversal(root.right);
+    }
+    var k := 1;
+    var j := |TreePreorderTraversal(root.left)|+1;
+    assert 0 <= k <= j <= |TreePreorderTraversal(root)| && TreePreorderTraversal(root.left) == TreePreorderTraversal(root)[1..|TreePreorderTraversal(root.left)|+1];
+
+    var s := 1+|TreePreorderTraversal(root.left)|;
+    var t := |TreePreorderTraversal(root)|;
+    assert 0 <= s <= t <= |TreePreorderTraversal(root)| && TreePreorderTraversal(root.right) == TreePreorderTraversal(root)[s..t];
+   }else if root.left != Nil && root.right == Nil {
+    calc {
+        TreePreorderTraversal(root);
+        [root]+TreePreorderTraversal(root.left);
+    }
+    var k := 1;
+    var j := |TreePreorderTraversal(root.left)|+1;
+    assert 0 <= k <= j <= |TreePreorderTraversal(root)| && TreePreorderTraversal(root.left) == TreePreorderTraversal(root)[1..j];
+   }else if root.left == Nil && root.right != Nil {
+    calc {
+        TreePreorderTraversal(root);
+        [root]+TreePreorderTraversal(root.right);
+    }
+    var k := 1;
+    var j := |TreePreorderTraversal(root.right)|+1;
+    assert 0 <= k <= j <= |TreePreorderTraversal(root)| && TreePreorderTraversal(root.right) == TreePreorderTraversal(root)[1..j];
+   }
+}
+
+lemma AllContained(root: Tree)
+    requires root != Nil
+    ensures forall x :: x in TreePreorderTraversal(root) ==> (x == root || x in TreePreorderTraversal(root.left) || x in TreePreorderTraversal(root.right))
+{
+    // tpt(root);
+    // NoNil(root);
+    // forall x | x in TreePreorderTraversal(root)
+    //     ensures x == root || x in TreePreorderTraversal(root.left) || x in TreePreorderTraversal(root.right)
+    // {
+    //     assert x != Nil;
+    //     if x == root {
+
+    //     }else if root.left != Nil && root.right != Nil {
+    //         calc {
+    //             TreePreorderTraversal(root);
+    //             [root]+TreePreorderTraversal(root.left)+TreePreorderTraversal(root.right);
+    //         }
+    //         assert x in [root]+TreePreorderTraversal(root.left)+TreePreorderTraversal(root.right);
+    //         assert x in TreePreorderTraversal(root.left) || x in TreePreorderTraversal(root.right);
+    //     }else if root.left == Nil && root.right != Nil {
+    //         calc {
+    //             TreePreorderTraversal(root);
+    //             [root]+TreePreorderTraversal(root.right);
+    //         }
+    //         assert x in [root]+TreePreorderTraversal(root.right);
+    //         assert x in TreePreorderTraversal(root.right);
+    //     }else if root.left != Nil && root.right == Nil {
+    //         calc {
+    //             TreePreorderTraversal(root);
+    //             [root]+TreePreorderTraversal(root.left);
+    //         }
+    //         assert x in [root]+TreePreorderTraversal(root.left);
+    //         assert x in TreePreorderTraversal(root.left);
+    //     }else{
+    //         assert false;
+    //     }
+
+    // }
+}
+
+lemma {:verify true} {:induction false} AllChildrenTraversalsAreSubstrings(root: Tree) 
+    requires root != Nil
+    ensures forall x ::x in TreePreorderTraversal(root) ==> isSubstring(TreePreorderTraversal(x), TreePreorderTraversal(root))
+{
+    NoNil(root);
+    AllContained(root);
+    forall x | x in TreePreorderTraversal(root) 
+        ensures isSubstring(TreePreorderTraversal(x), TreePreorderTraversal(root))
+    {
+        tpt(root);
+        if x == root {
+            var k, j := 0, |TreePreorderTraversal(root)|;
+            assert 0 <= k <= j <= |TreePreorderTraversal(root)| && TreePreorderTraversal(root) == TreePreorderTraversal(root)[k..j];
+        }else if x == root.left || x == root.right {
+           TreePreorderTraversalSubstrings(root); 
+        }else {
+            if root.left != Nil && root.right != Nil {
+                assert x != root;
+                assert TreePreorderTraversal(root) == [root] + TreePreorderTraversal(root.left) + TreePreorderTraversal(root.right);
+                if root.left != Nil  && x in TreePreorderTraversal(root.left) {
+                    AllChildrenTraversalsAreSubstrings(root.left);
+                    assert isSubstring(TreePreorderTraversal(x), TreePreorderTraversal(root.left));
+                    TreePreorderTraversalSubstrings(root);
+                    AllSubstringsAreSubstrings(TreePreorderTraversal(x), TreePreorderTraversal(root.left), TreePreorderTraversal(root));
+                }
+                if root.right != Nil && x in TreePreorderTraversal(root.right) {
+                    AllChildrenTraversalsAreSubstrings(root.right);
+                    assert isSubstring(TreePreorderTraversal(x), TreePreorderTraversal(root.right));
+                    TreePreorderTraversalSubstrings(root);
+                    AllSubstringsAreSubstrings(TreePreorderTraversal(x), TreePreorderTraversal(root.right), TreePreorderTraversal(root));
+                }
+            }else if root.left != Nil  && x in TreePreorderTraversal(root.left) {
+                AllChildrenTraversalsAreSubstrings(root.left);
+                assert isSubstring(TreePreorderTraversal(x), TreePreorderTraversal(root.left));
+                    TreePreorderTraversalSubstrings(root);
+                    AllSubstringsAreSubstrings(TreePreorderTraversal(x), TreePreorderTraversal(root.left), TreePreorderTraversal(root));
+            }else  if root.right != Nil && x in TreePreorderTraversal(root.right) {
+                AllChildrenTraversalsAreSubstrings(root.right);
+                    assert isSubstring(TreePreorderTraversal(x), TreePreorderTraversal(root.right));
+                    TreePreorderTraversalSubstrings(root);
+                    AllSubstringsAreSubstrings(TreePreorderTraversal(x), TreePreorderTraversal(root.right), TreePreorderTraversal(root));
+            }else{
+                assert x != root;
+                assert x !in TreePreorderTraversal(root.left);
+                assert x !in TreePreorderTraversal(root.right);
+                assert false;
+            }
+        }
+    }
+}
+
+lemma {:verify false} PreorderTraversalSubstrings(root: TreeNode)
+    requires root.Valid()
+    ensures root.left != null ==> isSubstring(PreorderTraversal(root.left), PreorderTraversal(root))
+    ensures root.right != null ==> isSubstring(PreorderTraversal(root.right), PreorderTraversal(root))
+{
+
+   if root.left != null && root.right != null {
+    calc {
+        PreorderTraversal(root);
+        [root]+PreorderTraversal(root.left)+PreorderTraversal(root.right);
+    }
+    var k := 1;
+    var j := |PreorderTraversal(root.left)|+1;
+    assert 0 <= k <= j <= |PreorderTraversal(root)| && PreorderTraversal(root.left) == PreorderTraversal(root)[1..|PreorderTraversal(root.left)|+1];
+
+    var s := 1+|PreorderTraversal(root.left)|;
+    var t := |PreorderTraversal(root)|;
+    assert 0 <= s <= t <= |PreorderTraversal(root)| && PreorderTraversal(root.right) == PreorderTraversal(root)[s..t];
+   }else if root.left != null && root.right == null {
+    calc {
+        PreorderTraversal(root);
+        [root]+PreorderTraversal(root.left);
+    }
+    var k := 1;
+    var j := |PreorderTraversal(root.left)|+1;
+    assert 0 <= k <= j <= |PreorderTraversal(root)| && PreorderTraversal(root.left) == PreorderTraversal(root)[1..j];
+   }else if root.left == null && root.right != null {
+    calc {
+        PreorderTraversal(root);
+        [root]+PreorderTraversal(root.right);
+    }
+    var k := 1;
+    var j := |PreorderTraversal(root.right)|+1;
+    assert 0 <= k <= j <= |PreorderTraversal(root)| && PreorderTraversal(root.right) == PreorderTraversal(root)[1..j];
+   }
+}
+
+// lemma AllChildrenTraversalsAreSubstrings(root: TreeNode) 
+//     requires root.Valid()
+//     ensures forall x :: x in root.repr && x in PreorderTraversal(root) ==> isSubstring(PreorderTraversal(x), PreorderTraversal(root))
+// {
+//     forall x | x in root.repr && x in PreorderTraversal(root) 
+//         ensures isSubstring(PreorderTraversal(x), PreorderTraversal(root))
+//     {
+//         if x == root {
+
+//         }else if x == root.left || x == root.right {
+//            PreorderTraversalSubstrings(root); 
+//         }else {
+//             if root.left != null && x in root.left.repr {
+//                 AllChildrenTraversalsAreSubstrings(root.left);
+//             }
+//             if root.right != null && x in root.right.repr {
+//                 AllChildrenTraversalsAreSubstrings(root.right);
+//             }
+//         }
+//     }
+// }
+
+predicate seqElement<A>(s: seq<A>, elem: A, k: nat)
+
+{
+    0 <= k < |s| && elem in s && s[k] == elem
+}
+
+lemma {:verify } PreorderTraversalChildrenAreLater1(root: TreeNode)
+    requires root.Valid()
+    //would not verify until asserted that x was also in PreorderTraversal(root)
+    ensures forall x :: x in root.repr && x in PreorderTraversal(root) ==> exists k: nat :: 0 <= k < |PreorderTraversal(root)| && PreorderTraversal(root)[k] == x
+{
+    forall x | x in root.repr 
+        ensures exists k: nat :: 0 <= k < |PreorderTraversal(root)| && PreorderTraversal(root)[k] == x
+    {
+        assert x in PreorderTraversal(root);
+        seqbusiness(PreorderTraversal(root), x);
+    }
+}
+
+lemma {:verify true} PreorderTraversalChildrenAreLater(root: TreeNode)
+    requires root.Valid()
+    //the following does not verify
+    ensures forall x :: x in root.repr && x in PreorderTraversal(root) && x != root ==> exists k: nat :: 0 < k < |PreorderTraversal(root)| && PreorderTraversal(root)[k] == x
+{
+    
+    // forall x | x in root.repr && x in PreorderTraversal(root) && x != root
+        // ensures exists k: nat :: 0 < k < |PreorderTraversal(root)| && PreorderTraversal(root)[k] == x
+    // {
+        // PreorderTraversalChildrenAreLater1(root);
+        // var k :| 0 <= k < |PreorderTraversal(root)| && PreorderTraversal(root)[k] == x;
+        // assert PreorderTraversal(root)[0] == root;
+    // }
+    // but it verifies here, at least I get the green checkmark
+    // assert forall x :: x in root.repr ==> exists k: nat :: 0 <= k < |PreorderTraversal(root)| && PreorderTraversal(root)[k] == x;
+}
+
+lemma {:verify false} TreePreorderTraversalChildrenAreLater3(root: Tree, elem: Tree, k: nat) 
+    requires elem in TreePreorderTraversal(root)
+    requires TreePreorderTraversal(root)[k] == elem
+    // ensures forall child :: child in TreePreorderTraversal(elem) && child in PreorderTraversal(root) && child != elem ==> exists j: nat :: k < j < |PreorderTraversal(root)| && PreorderTraversal(root)[j] == child
+{
+
+}
+
+
+
+lemma {:verify false} PreorderTraversalChildrenAreLater3(root: TreeNode, elem: TreeNode, k: nat) 
+    requires root.Valid()
+    requires elem in root.repr
+    requires elem in PreorderTraversal(root)
+    requires PreorderTraversal(root)[k] == elem
+    // ensures forall child :: child in elem.repr && child in PreorderTraversal(root) && child != elem ==> exists j: nat :: k < j < |PreorderTraversal(root)| && PreorderTraversal(root)[j] == child
+{
+
+}
+
+lemma seqbusiness<A>(s: seq<A>, elem: A)
+    requires elem in s
+    ensures exists k:nat :: 0 <= k < |s| && s[k] == elem
+    ensures exists k:nat :: seqElement(s, elem, k) 
+{
+    assert elem in s;
+    assert exists k:nat :: 0 <= k < |s| && s[k] == elem && seqElement(s, elem, k);
+}
+
+method swapChildren(root: TreeNode) returns (newRoot: TreeNode)
+    modifies root
+    requires root.Valid()
+    ensures root == newRoot && newRoot.Valid()
+    ensures root.right == old(root.left) && root.left == old(root.right)
+    ensures forall x :: x in root.repr && x != root ==> unchanged(x)
+{
+
+    var temp := root.left;
+    root.left := root.right;
+    root.right := temp;
+    return root;
 }
 
 method  invertBinaryTree(root: TreeNode?) returns (newRoot: TreeNode?)
@@ -116,6 +441,177 @@ method  invertBinaryTree(root: TreeNode?) returns (newRoot: TreeNode?)
     }else{
         return null;
     }
+}
+
+lemma ChildNodesAreInRoot(root: TreeNode, child: TreeNode)
+    requires root.Valid()
+    requires (root.left != null && child == root.left) || (root.right != null && root.right == child)
+    ensures child in root.repr;
+{
+
+}
+
+lemma ChildChildrenNodesAreInRoot(root: TreeNode, child: TreeNode)
+    requires root.Valid()
+    requires (root.left != null && (child == root.left.left || child == root.left.right)) || (root.right != null && (root.right.left == child || root.right.right == child))
+    ensures child in root.repr;
+{
+
+}
+
+lemma ChildNodesAreValid(root: TreeNode, child: TreeNode)
+    requires root.Valid()
+    requires child in root.repr;
+    decreases root.repr
+    ensures child.repr <= root.repr;
+    ensures child.Valid()
+{
+    if child == root {
+    }else if child == root.left {
+
+    }else if child == root.right {
+
+    }else if root.left != null && root.right != null {
+        assert root.repr == {root} + root.left.repr + root.right.repr;
+        if child in root.left.repr {
+            ChildNodesAreValid(root.left, child);
+        }else if child in root.right.repr {
+            ChildNodesAreValid(root.right, child);
+        }else{
+            assert false;
+        }
+    }else if root.right != null {
+
+    }else if root.left != null {
+
+    }else{
+        assert false;
+    }
+}
+
+twostate lemma ValidSwappingStillValid(root: TreeNode, child: TreeNode)
+    requires root.Valid()
+    requires child in root.repr;
+    requires child.left == old(child.right) && child.right == old(child.left)
+    ensures root.Valid()
+{
+    ChildNodesAreValid(root,child);
+    assert child.Valid();
+}
+
+function TreeUnion(nodes: seq<TreeNode>): set<TreeNode>
+    reads set x | 0 <= x < |nodes| :: nodes[x]
+{
+   if |nodes| > 0 then nodes[0].repr + TreeUnion(nodes[1..]) else {}
+}
+//fresh ensures that a variable was initialized by a method or two-state function
+
+method {:verify false} invertBinaryTreeIterative1(root: TreeNode?) returns (newRoot: TreeNode?)
+    modifies if root != null then root.repr else {}
+    requires root != null ==> root.Valid()
+    ensures root == null ==> newRoot == null
+    ensures root != null ==> newRoot == root && newRoot.repr == old(root.repr)
+    // ensures root != null ==> newRoot != null && newRoot.repr == old(root.repr) && newRoot.Valid()
+    // ensures root != null ==> forall node :: node in newRoot.repr ==> node.right == old(node.left) && node.left == old(node.right)
+    // ensures root != null ==> newRoot == root && newRoot.right == old(root.left) && root.left == old(root.right)
+{
+    if root == null {
+        return null;
+    }
+
+    var nodes := PreorderTraversal(root);
+    assert forall k :: 0 <= k < |nodes| ==> nodes[k] in root.repr && nodes[k].Valid();
+    ghost var visited: set<TreeNode> := {};
+    ghost var unvisited: set<TreeNode> := root.repr;
+    var i := 0;
+    while i < |nodes| 
+        modifies root.repr
+        invariant 0 <= i <= |nodes|
+        invariant root.repr == old(root.repr)
+        invariant forall k::i < k <= |nodes| ==> unchanged(nodes[k])
+    //     // invariant visited == set k | k < i < |nodes| :: nodes[k]
+    //     invariant forall x :: x in nodes ==> x.Valid()
+    //     // invariant root.Valid()
+    //     // invariant forall k :: 0<= k < i ==> nodes[k].right == old(nodes[k].left) && nodes[k].left == old(nodes[k].right)
+    {
+        assert nodes[i] in nodes;
+        assert nodes[i] in root.repr;
+        assert nodes[i].Valid();
+    // //     var temp := nodes[i].left;
+    // //     nodes[i].left := nodes[i].right;
+    // //     nodes[i].right := temp;
+        nodes[i].left, nodes[i].right := nodes[i].right, nodes[i].left;
+        assert nodes[i].right == old(nodes[i].left) && nodes[i].left == old(nodes[i].right);
+    // //     // var newNode := swapChildren(nodes[i]);
+    // //     ValidSwappingStillValid(root, nodes[i]);
+    // //     visited := visited + {nodes[i]};
+        i := i + 1;
+    }
+    return root;
+}
+
+method {:verify false} invertBinaryTreeIterative(root: TreeNode?) returns (newRoot: TreeNode?)
+    modifies if root != null then root.repr else {}
+    requires root != null ==> root.Valid()
+    ensures root == null ==> newRoot == null
+    // ensures root != null ==> newRoot != null && newRoot.repr == old(root.repr) && newRoot.Valid()
+    // ensures root != null ==> newRoot == root && newRoot.right == old(root.left) && root.left == old(root.right)
+    ensures newRoot.repr == old(root.repr)
+    ensures root != null ==> newRoot == root
+    // ensures root != null ==> forall node :: node in newRoot.repr ==> node.right == old(node.left) && node.left == old(node.right)
+{
+    if root == null {
+        return null;
+    }
+    assert root != null;
+    assert root.Valid();
+    var stack: seq<TreeNode> := [root];
+    ghost var visited: set<TreeNode> := {};
+    ghost var unvisited: set<TreeNode> := root.repr;
+    assert TreeUnion(stack) == unvisited;
+    assert TreeUnion(stack) == root.repr - visited;
+    assert root in root.repr;
+    assert root.repr <= root.repr;
+    assert root in stack;
+    while |stack| > 0 
+        modifies root.repr
+        invariant root.Valid()
+        invariant root.repr == old(root.repr)
+        invariant forall x :: x in stack ==> x in root.repr;
+        invariant forall x :: x in unvisited ==> unchanged(x)
+        // invariant forall x :: x in stack ==> x.Valid() && x.repr <= root.repr;
+        invariant visited + unvisited == root.repr;
+        // invariant visited == visited + {stack[0]}
+        // invariant TreeUnion(stack) == root.repr - visited
+        invariant forall node :: node in visited ==> node.right == old(node.left) && node.left == old(node.right) && node.Valid()
+        decreases unvisited
+    {
+        var current: TreeNode := stack[0];
+        assert current in stack;
+        ChildNodesAreValid(root, current);
+        if current.left != null {
+            assert current.left.repr <= root.repr;
+            assert current.left in root.repr;
+            ChildNodesAreValid(root, current.left);
+            stack :=  stack + [current.left];
+        }
+        if current.right != null {
+            assert current.right.repr <= root.repr;
+            assert current.right in root.repr;
+            ChildNodesAreValid(root, current.right);
+            stack := stack + [current.right];
+        }
+        var temp := current.left;
+        current.left := current.right;
+        current.right := temp;
+        assert temp == old(current.left);
+        assert current.left == old(current.right) && current.right == old(current.left);
+        ValidSwappingStillValid(root, current);
+        visited := visited + {current};
+        unvisited := unvisited - {current};
+        stack := stack[1..];
+    }
+    return root;
 }
         // assert root.right == old(root.left) && root.left == old(root.right);
         // if root.right != null && root.left != null {
