lib/seq.dfy
@@ -1,0 +1,103 @@
+
+module Seq {
+    predicate substring1<A>(sub: seq<A>, super: seq<A>) {
+        exists k :: 0 <= k < |super| && sub <= super[k..]
+    }
+
+
+    predicate isSubstringAlt<A(!new)>(sub: seq<A>, super: seq<A>) {
+        |sub| <= |super| && exists xs: seq<A> :: IsSuffix(xs, super) && sub <= xs
+    }
+
+    predicate isSubstring<A>(sub: seq<A>, super: seq<A>) {
+        |sub| <= |super| && exists k,j :: 0 <= k < j <= |super| && sub == super[k..j]
+    }
+
+    lemma SliceOfSliceIsSlice<A>(xs: seq<A>, k: int, j: int, s: int, t: int)
+        requires 0 <= k <= j <= |xs|
+        requires 0 <= s <= t <= j-k
+        ensures xs[k..j][s..t] == xs[(k+s)..(k+s+(t-s))]
+    {
+        // if k == 0 && j == 0 {
+        //     assert xs[k..j] == [];
+        //     assert xs[k..j][s..t] == [];
+        // }else if k == 0 && j == |xs| {
+        //     assert xs[k..j] == xs;
+        //     assert xs[k..j][s..t] == xs[(k+s)..(k+s+t-s)];
+        // }else if k == |xs| && j == |xs| {
+        //     assert xs[k..j] == [];
+        //     assert xs[k..j][s..t] == xs[(k+s)..(k+s+t-s)];
+        // }else 
+        if 0 <= k <= j <= |xs| {
+            if j-k == 0 {
+
+            }else if t-s == 0 {
+
+            }else if t-s > 0 {
+                SliceOfSliceIsSlice(xs, k, j, s,t-1);
+                assert xs[k..j][s..t] == xs[k..j][s..(t-1)]+[xs[k..j][t-1]];
+            }
+        }else{
+            assert false;
+        }
+    }
+
+    lemma AllSubstringsAreSubstrings<A>(subsub: seq<A>, sub: seq<A>, super: seq<A>)
+        requires isSubstring(sub, super)
+        requires isSubstring(subsub, sub)
+        ensures isSubstring(subsub, super)
+    {
+        assert |sub| <= |super|;
+        assert |subsub| <= |super|;
+        var k,j :| 0 <= k < j <= |super| && sub == super[k..j];
+        var s,t :| 0 <= s < t <= |sub| && subsub == sub[s..t];
+        assert t <= (j-k) <= j;
+        //[3,4,5,6,7,8,9,10,11,12,13][2,7] //k,j
+        //[5,6,7,8,9,10][1..3] //s,t
+        //[5,7,8]
+        // var example:= [3,4,5,6,7,8,9,10,11,12,13];
+        // assert example[2..7] == [5,6,7,8,9];
+        // assert example[2..7][1..3] == [6,7];
+        // assert example[3..5] == [6,7];
+        // assert k+s+(t-s)
+        // assert 2+1+(3-1) == 5;
+        /*
+        assert s[..idx] == [s[0]] + s[1..idx];
+        assert s[1..idx] == s[1..][..(idx-1)];
+        assert s[1..][(idx-1)..] == s[idx..];
+        */
+        assert super[..j][..t] == super[..(t)];
+        assert super[k..][s..] == super[(k+s)..];
+        if t < j {
+            calc {
+                subsub;
+                super[k..j][s..t];
+                {SliceOfSliceIsSlice(super,k,j,s,t);}
+                super[(k+s)..(k+s+(t-s))];
+            }
+        } else if t <= j {
+
+        }
+        var z,q :| 0 <= z <= q <= |super| && super[z..q] == super[k..j][s..t];
+    }
+
+
+    predicate IsSuffix<T>(xs: seq<T>, ys: seq<T>) {
+        |xs| <= |ys| && xs == ys[|ys| - |xs|..]
+    }
+
+    predicate IsSuffix2<T>(xs: seq<T>, ys: seq<T>) {
+        |xs| <= |ys| && exists K :: 0 <= K <= |ys|-|xs| && ys == ys[0..K] + xs + ys[(K+|xs|)..]
+    }
+
+    method Test() {
+        var t1 := [4,5,6,1,2,3];
+        // assert t1 == [4,5,6]+[1,2,3];
+        var s1 := [1,2,3];
+        assert IsSuffix(s1,t1);
+        // assert isSubstring(s1,t1);
+        assert substring1(s1, t1);
+
+    }
+
+}
